rename dynamic_redblack_btree.v to dynamic_redblack.v

dynamic_redblack.v
@@ -7,6 +7,12 @@ Set Implicit Arguments.
 Unset Strict Implicit.
 Unset Printing Implicit Defensive.
 
+Ltac decompose_rewrite :=
+  let H := fresh "H" in
+  case/andP || (move=>H; rewrite ?H ?(eqP H)).
+
+Ltac decomp ok := move: ok => /=; repeat decompose_rewrite.
+
 Section btree.
 
 Variables D A : Type.
@@ -19,20 +25,64 @@ Inductive btree : Type :=
 
 End btree.
 
-Ltac decompose_rewrite :=
-  let H := fresh "H" in
-  case/andP || (move=>H; rewrite ?H ?(eqP H)).
+Section eq_btree.
+
+Definition eq_color c1 c2 :=
+  match c1,c2 with
+  | Black,Black | Red,Red => true
+  | _,_ => false
+  end.
+
+Lemma color_eqP : Equality.axiom eq_color.
+Proof.
+  move; case; case => /=;
+  try apply ReflectT => //;
+  apply ReflectF => //. 
+Qed.
+
+Canonical color_eqMixin := EqMixin color_eqP.
+Canonical color_eqType := Eval hnf in EqType color color_eqMixin.
+
+Variables D A : eqType.
+
+Fixpoint eq_btree (t1 t2 : btree D A) := 
+  match t1,t2 with
+  | Bleaf a, Bleaf b => a == b
+  | Bnode c1 l1 d1 r1, Bnode c2 l2 d2 r2 =>
+    (d1 == d2) && (c1 == c2) && (eq_btree l1 l2) && (eq_btree r1 r2)
+  | Bnode _ _ _ _, Bleaf _ 
+  | Bleaf _, Bnode _ _ _ _ => false
+  end.
+
+Lemma eq_dtree_refl (t : btree D A) : eq_btree t t.
+Proof. elim t => [? l H1 ? r H2 /=|a //=]; by rewrite H1 H2 !eq_refl. Qed.
+
+Lemma eq_dtree_iff t1 t2 : t1 = t2 <-> eq_btree t1 t2.
+Proof.
+  split => [->|]; first by rewrite eq_dtree_refl.
+  move: t1 t2; elim => [? l1 lH1 ? r1 rH1|?]; elim => [? l2 lH2 ? r2 rH2 H|?] //;
+  last by move/eqP => /= ->.
+  move/andP: H; case; move/andP; case; move/andP; case; move/eqP => ->; move/eqP => -> H1 H2.
+  by rewrite (lH1 _ H1) (rH1 _ H2).
+Qed.
+
+Lemma btree_eqP : Equality.axiom eq_btree.
+Proof.
+  move; case => [? l1 ? r1 |?]; case => [? l2 ? r2|?] //;
+  set b:= (eq_btree _ _); case Hb : b; subst b;
+  try (apply ReflectT; apply eq_dtree_iff => //); try apply ReflectF => //.
+   by case => H1 H2 H3 H4; move: Hb; rewrite H1 H2 H3 H4 eq_dtree_refl.
+  by case => H1; move: Hb; rewrite H1 eq_dtree_refl.
+Qed.
+
+Canonical btree_eqMixin := EqMixin btree_eqP.
+Canonical btree_eqType := Eval hnf in EqType (btree D A) btree_eqMixin.
+
+End eq_btree.
 
 Section dtree.
 
-(*
-Variable w : nat.
-Hypothesis Hw : w >= 2.
-*)
-
 Definition dtree := btree (nat * nat) (seq bool).
-
-Definition empty_tree : dtree := Bleaf _ [::].
 
 Fixpoint daccess (B : dtree) (i : nat) :=
   match B with
@@ -83,68 +133,10 @@ Fixpoint dones (B : dtree) :=
   | Bleaf s => count_mem true s
   end.
 
-Definition rbnode c l r := Bnode c l (dsize l, dones l) r.
-
-Definition bnode l r := Bnode Black l (dsize l, dones l) r.
-
-Definition rnode l r := Bnode Red l (dsize l, dones l) r.
-
-Definition leaf a : dtree := Bleaf _ a.
-
-Definition eq_color c1 c2 :=
-  match c1,c2 with
-  | Black,Black | Red,Red => true
-  | _,_ => false
-  end.
-
-Lemma color_eqP : Equality.axiom eq_color.
-Proof.
-  move; case; case => /=;
-  try apply ReflectT => //;
-  apply ReflectF => //. 
-Qed.
-
-Canonical color_eqMixin := EqMixin color_eqP.
-Canonical color_eqType := Eval hnf in EqType color color_eqMixin.
-
-Fixpoint eq_dtree (t1 t2 : dtree) := 
-  match t1,t2 with
-  | Bleaf a, Bleaf b => a == b
-  | Bnode c1 l1 d1 r1, Bnode c2 l2 d2 r2 =>
-    (d1 == d2) && (c1 == c2) && (eq_dtree l1 l2) && (eq_dtree r1 r2)
-  | Bnode _ _ _ _, Bleaf _ 
-  | Bleaf _, Bnode _ _ _ _ => false
-  end.
-
-Lemma eq_dtree_refl (t : dtree) : eq_dtree t t.
-Proof. elim t => [? l H1 ? r H2 /=|a //=]; by rewrite H1 H2 !eq_refl. Qed.
-
-Lemma eq_dtree_iff t1 t2 : t1 = t2 <-> eq_dtree t1 t2.
-Proof.
-  split => [->|]; first by rewrite eq_dtree_refl.
-  move: t1 t2; elim => [? l1 lH1 ? r1 rH1|?]; elim => [? l2 lH2 ? r2 rH2 H|?] //;
-  last by move/eqP => /= ->.
-  move/andP: H; case; move/andP; case; move/andP; case; move/eqP => ->; move/eqP => -> H1 H2.
-  by rewrite (lH1 _ H1) (rH1 _ H2).
-Qed.
-
-Lemma dtree_eqP : Equality.axiom eq_dtree.
-Proof.
-  move; case => [? l1 ? r1 |?]; case => [? l2 ? r2|?] //;
-  set b:= (eq_dtree _ _); case Hb : b; subst b;
-  try (apply ReflectT; apply eq_dtree_iff => //); try apply ReflectF => //.
-   by case => H1 H2 H3 H4; move: Hb; rewrite H1 H2 H3 H4 eq_dtree_refl.
-  by case => H1; move: Hb; rewrite H1 eq_dtree_refl.
-Qed.
-
-Canonical dtree_eqMixin := EqMixin dtree_eqP.
-Canonical dtree_eqType := Eval hnf in EqType dtree dtree_eqMixin.
 
 Definition access (s : seq bool) i := nth false s i.
 
 Variables low high : nat.  (* (w ^ 2)./2 and (w ^ 2).*2 *)
-Hypothesis Hlow : low <= high./2.
-Hypothesis Hhigh : 1 < high.
 
 Fixpoint wf_dtree (B : dtree) :=
   match B with
@@ -229,373 +221,396 @@ Corollary drank_all (B : dtree) :
   wf_dtree B -> drank B (dsize B) = (count_mem true) (dflatten B).
 Proof. move => wf. by rewrite drankE // /rank dsizeE // take_size. Qed.
 
-Section insert.
+Definition drank_size B := drank B (dsize B).
 
-  Definition drank_size B := drank B (dsize B).
-
-  Definition balance col (l : dtree) (r : dtree) : dtree :=
-    match col with
-    | Red => Bnode Red l (dsize l, drank_size l) r
-    | Black => match l, r with
-               | Bnode Red (Bnode Red a _ b) _ c, d
-               | Bnode Red a _ (Bnode Red b _ c), d
-               | a, Bnode Red (Bnode Red b _ c) _ d
-               | a, Bnode Red b _ (Bnode Red c _ d)
-                 => Bnode Red (Bnode Black a (dsize a, drank_size a) b)
-                          (dsize a + dsize b, drank_size a + drank_size b)
-                          (Bnode Black c (dsize c, drank_size c) d)
-               | _, _ => Bnode Black l (dsize l, drank_size l) r
-               end
-    end.
-
-  Definition balanceL col (l : dtree) (r : dtree) : dtree :=
-    match col with
-    | Red => Bnode Red l (dsize l, dones l) r
-    | Black => match l with
-               | Bnode Red (Bnode Red a _ b) _ c
-               | Bnode Red a _ (Bnode Red b _ c)
-                   => Bnode Red (Bnode Black a (dsize a, dones a) b)
-                          (dsize a + dsize b, dones a + dones b)
-                          (Bnode Black c (dsize c, dones c) r)
-               | _ => Bnode Black l (dsize l, dones l) r
-               end
-    end.
-
-  Definition balanceR col (l : dtree) (r : dtree) : dtree :=
-    match col with
-    | Red => Bnode Red l (dsize l, dones l) r
-    | Black => match r with
-               | Bnode Red (Bnode Red b _ c) _ d
-               | Bnode Red b _ (Bnode Red c _ d)
-                   => Bnode Red (Bnode Black l (dsize l, dones l) b)
-                          (dsize l + dsize b, dones l + dones b)
-                          (Bnode Black c (dsize c, dones c) d)
-               | _ => Bnode Black l (dsize l, dones l) r
-               end
-    end.
-
-  Definition dins_leaf s b i :=
-    let s' := insert1 s b i in
-    if size s + 1 == high
-    then let n  := (size s') %/ 2 in
-         let sl := take n s' in
-         let sr := drop n s' in
-         Bnode Red (Bleaf _ sl) (size sl, count_mem true sl) (Bleaf _ sr)
-    else Bleaf _ s'.
-
-  Fixpoint dins (B : dtree) b i : dtree :=
-    match B with
-    | Bleaf s => dins_leaf s b i
-    | Bnode c l (num, ones) r =>
-      if i < num
-      then balanceL c (dins l b i) r
-      else balanceR c l (dins r b (i - num))
-    end.
-
-  Definition dinsert (B : dtree) b i : dtree :=
-    match dins B b i with
-    | Bleaf s => Bleaf _ s
-    | Bnode _ l d r => Bnode Black l d r
-    end.
-
-  (* Correctness lemmas *)
-
-  Lemma dflatten_node c l d r :
-    dflatten (Bnode c l d r) = dflatten l ++ dflatten r.
-  Proof. by []. Qed.
-
-  Lemma balanceE c l r : dflatten (balance c l r) = dflatten l ++ dflatten r.
-  Proof.
-    rewrite /balance. case: c. exact: dflatten_node.
-    case: l => [[[[] lll llD llr|llA] lD [[] lrl lrD lrr|lrA]|ll lD lr]|lA] /=;
-    case: r => [[[[] rll rlD rlr|rlA] rD [[] rrl rrD rrr|rrA]|rl rD rr]|rA] /=;
-      try done; by rewrite !catA.
-  Qed.
-
-  Lemma balanceLE c l r : dflatten (balanceL c l r) = dflatten l ++ dflatten r.
-  Proof.
-    rewrite /balanceL. case: c. exact: dflatten_node.
-    case: l => [[[[] lll llD llr|llA] lD [[] lrl lrD lrr|lrA]|ll lD lr]|lA] //=;
-      by rewrite !catA.
-  Qed.
-
-  Lemma balanceRE c l r : dflatten (balanceR c l r) = dflatten l ++ dflatten r.
-  Proof.
-    rewrite /balanceR. case: c. exact: dflatten_node.
-    case: r => [[[[] rll rlD rlr|rlA] rD [[] rrl rrD rrr|rrA]|rl rD rr]|rA] //=;
-      by rewrite !catA.
-  Qed.
-
-  (* Well-foundedness lemmas
-   * Show that dinsert always returns a well-founded tree
-   *)
-
-  Lemma balanceL_wf c (l r : dtree) :
-    wf_dtree l -> wf_dtree r -> wf_dtree (balanceL c l r).
-  Proof.
-    case: c => /= wfl wfr.
-      by rewrite wfl wfr ?(dsizeE,donesE,eqxx).
-    case: l wfl =>
-      [[[[] lll [lln llo] llr|llA] [ln lo] [[] lrl [lrn lro] lrr|lrA]
-       |ll [ln lo] lr]|lA] /=;
-      rewrite wfr; repeat decompose_rewrite;
-      by rewrite ?(dsizeE,donesE,size_cat,count_cat,eqxx).
-  Qed.
-
-  Lemma balanceR_wf c (l r : dtree) :
-    wf_dtree l -> wf_dtree r -> wf_dtree (balanceR c l r).
-  Proof.
-    case: c => /= wfl wfr.
-      by rewrite wfl wfr ?(dsizeE,donesE,eqxx).
-    case: r wfr => [[[[] rll [rln rlo] rlr|rlA] [rn ro] [[] rrl
-                             [rrn rro] rrr|rrA]|rl [rn ro] rr]|rA] /=;
-      rewrite wfl; repeat decompose_rewrite;
-      by rewrite ?(dsizeE,donesE,size_cat,count_cat,eqxx).
-  Qed.
-End insert.
 End dtree.
 
-Section insert_prop.
-  Variables low high : nat.
-  Local Notation dins := (dins high).
-  Local Notation dins_leaf := (dins_leaf high).
-  Local Notation dinsert := (dinsert high).
 
-  Hypothesis Hlow : low.*2 <= high.
-  Hypothesis Hhigh : 1 < high.
-  Definition wf_dtree' t :=
-    if t is Bleaf s then size s < high else wf_dtree low high t.
+Section insert.
+Variables D A : Type.
+Variable mkD : btree D A -> D.
 
-  Lemma wf_dtree_dtree' t : wf_dtree low high t -> wf_dtree' t.
-  Proof. by case: t => //= s /andP[_ ->]. Qed.
+Definition balance col (l r : btree D A) : btree D A :=
+  match col with
+  | Red => Bnode Red l (mkD l) r
+  | Black => match l, r with
+             | Bnode Red (Bnode Red a _ b) _ c, d
+             | Bnode Red a _ (Bnode Red b _ c), d
+             | a, Bnode Red (Bnode Red b _ c) _ d
+             | a, Bnode Red b _ (Bnode Red c _ d) =>
+               let l := Bnode Black a (mkD a) b in
+               Bnode Red l (mkD l) (Bnode Black c (mkD c) d)
+             | _, _ => Bnode Black l (mkD l) r
+             end
+  end.
 
-  Lemma wf_dtree'_dtree t : wf_dtree' t -> wf_dtree 0 high t.
-  Proof.
-    elim: t => //= c l IHl [n o] r IHr; repeat decompose_rewrite => /=.
-    by rewrite !(IHl,IHr,wf_dtree_dtree').
-  Qed.
+Definition balanceL col (l r : btree D A) : btree D A :=
+  match col with
+  | Red => Bnode Red l (mkD l) r
+  | Black => match l with
+             | Bnode Red (Bnode Red a _ b) _ c
+             | Bnode Red a _ (Bnode Red b _ c) =>
+               let l := Bnode Black a (mkD a) b in
+               Bnode Red l (mkD l) (Bnode Black c (mkD c) r)
+             | _ => Bnode Black l (mkD l) r
+             end
+  end.
 
-  Lemma wf_dtree'_node c l d r :
-    wf_dtree' (Bnode c l d r) = wf_dtree low high (Bnode c l d r). 
-  Proof. by []. Qed.
+Definition balanceR col (l r : btree D A) : btree D A :=
+  match col with
+  | Red => Bnode Red l (mkD l) r
+  | Black => match r with
+             | Bnode Red (Bnode Red b _ c) _ d
+             | Bnode Red b _ (Bnode Red c _ d) =>
+               let lb := Bnode Black l (mkD l) b in
+               Bnode Red lb (mkD lb) (Bnode Black c (mkD c) d)
+             | _ => Bnode Black l (mkD l) r
+             end
+  end.
 
-  Lemma leq_half n : n./2 <= n.
-  Proof. by rewrite -{2}(odd_double_half n) -addnn addnA leq_addl. Qed.
+Variable bins_leaf : A -> bool -> nat -> btree D A.
+Variable lt_index : nat -> D -> bool.
+Variable right_index : nat -> D -> nat.
 
-  Lemma dins_leaf_wf s b i : size s < high -> wf_dtree' (dins_leaf s b i).
-  Proof.
-    move=> Hs.
-    rewrite /dins_leaf addn1 divn2.
-    case: ifP => Hsize /=.
-      rewrite ?(eqxx,size_insert1,(eqP Hsize),size_drop,size_takel,leq_half) //.
-      have:= half_leq Hlow; rewrite doubleK => Hlow'.
-      set hhigh := high./2.
-      rewrite Hlow' -(odd_double_half high) -addnn addnA addnK.
-      have Hup : 0 < odd high + high./2.
-        by rewrite -addn1 leq_add // (half_leq Hhigh).
-      rewrite -add1n leq_add // (leq_trans Hlow' (leq_addl _ _)).
+Fixpoint bins (B : btree D A) b i : btree D A :=
+  match B with
+  | Bleaf s => bins_leaf s b i
+  | Bnode c l d r =>
+      if lt_index i d
+      then balanceL c (bins l b i) r
+      else balanceR c l (bins r b (right_index i d))
+    end.
+
+Definition binsert (B : btree D A) b i : btree D A :=
+  match bins B b i with
+  | Bleaf s => Bleaf _ s
+  | Bnode _ l d r => Bnode Black l d r
+  end.
+
+(*
+ * Following Appel (2011), pp. 6 - 8
+ *
+ * ctxt = "color context", or the color of
+ * the parent node
+ *
+ * bh = "black height", i.e. # of black nodes on the
+ * path from the root
+ *)
+Fixpoint is_redblack (B : btree D A) ctxt bh :=
+  match B with
+  | Bleaf _ => bh == 0
+  | Bnode c l _ r =>
+    match c, ctxt with
+    | Red, Red => false
+    | Red, Black => is_redblack l Red bh
+                    && is_redblack r Red bh
+    | Black, _ => (bh > 0) && is_redblack l Black (bh.-1) &&
+                              is_redblack r Black (bh.-1)
+    end
+  end.
+
+Definition nearly_redblack B bh :=
+  match B with
+  | Bnode Red l _ r => is_redblack l Black bh && is_redblack r Black bh
+  | _ => is_redblack B Black bh
+  end.
+
+Hypothesis Hbins_leaf : forall a b i, is_redblack (bins_leaf a b i) Black 0.
+
+Lemma is_redblack_Red_Black B n :
+  is_redblack B Red n -> is_redblack B Black n.
+Proof. by case: B => /= [[]|]. Qed.
+
+Lemma balanceL_Black_nearly_is_redblack l r n :
+  nearly_redblack l n -> is_redblack r Black n ->
+  is_redblack (balanceL Black l r) Black n.+1.
+Proof.
+  case: l => [[[[] lll ? llr|?] ? [[] lrl ? lrr|?]|ll ? lr]|?] /=;
+    repeat decompose_rewrite => //;
+    by rewrite !is_redblack_Red_Black -?(eqP H1).
+Qed.
+
+Lemma balanceR_Black_nearly_is_redblack l r n :
+  nearly_redblack r n -> is_redblack l Black n ->
+  is_redblack (balanceR Black l r) Black n.+1.
+Proof.
+  case: r => [[[[] rll ? rlr|?] ? [[] rrl ? rrr|?]|rl ? rr]|?] /=;
+    repeat decompose_rewrite => //;
+    by rewrite !is_redblack_Red_Black -?(eqP H1).
+Qed.
+
+Lemma is_redblack_nearly_redblack B c n :
+  is_redblack B c n -> nearly_redblack B n.
+Proof.
+  case: B => //= -[]; case: c => // l p r /andP [Hl Hr].
+  by rewrite !is_redblack_Red_Black.
+Qed.
+
+Lemma bins_is_redblack B b i n :
+  (is_redblack B Black n -> nearly_redblack (bins B b i) n) /\
+  (is_redblack B Red n -> is_redblack (bins B b i) Black n).
+Proof.
+  elim: B i n => [c l IHl d r IHr | a] i n; last first.
+    split => /= /eqP -> //; by apply: is_redblack_nearly_redblack.
+  have Hbk : is_redblack (Bnode Black l d r) Black n ->
+             is_redblack (bins (Bnode Black l d r) b i) Black n.
+  rewrite {3}[Black]lock /= -lock => /andP [/andP [/prednK <- Hl] Hr].
+    case: ifP => Hi.
+      rewrite balanceL_Black_nearly_is_redblack //; by apply IHl.
+    rewrite balanceR_Black_nearly_is_redblack //; by apply IHr.
+  split; case: c => //.
+  + move=> /= /andP [Hl Hr].
+    case: ifP => Hi /=; [move: Hr | move: Hl] => /is_redblack_Red_Black ->;
+      rewrite /= ?andbT; by [apply IHl | apply IHr].
+  + move/Hbk; by apply is_redblack_nearly_redblack.
+Qed.
+
+Definition is_red D A (B : btree D A) :=
+  if B is Bnode Red _ _ _ then true else false.
+
+Lemma binsert_is_redblack B b i n :
+  is_redblack B Red n ->
+  is_redblack (binsert B b i) Red (n + is_red (bins B b i)).
+Proof.
+  move/(proj2 (bins_is_redblack _ b i _)).
+  rewrite /binsert addnC.
+  destruct bins => //=.
+  case: c => //= /andP [Hd1 Hd2].
+  by rewrite !is_redblack_Red_Black.
+Qed.
+
+Corollary binsert_is_redblack' B b i n :
+  is_redblack B Red n -> exists n', is_redblack (binsert B b i) Red n'.
+Proof. esplit; apply /binsert_is_redblack /H. Qed.
+
+End insert.
+
+Section dinsert.
+
+Variables low high : nat.  (* (w ^ 2)./2 and (w ^ 2).*2 *)
+Hypothesis Hlow : low.*2 <= high.
+Hypothesis Hhigh : 1 < high.
+
+Definition mkD l := (dsize l, dones l).
+Local Notation balance := (balance mkD).
+Local Notation balanceL := (balanceL mkD).
+Local Notation balanceR := (balanceR mkD).
+Local Notation wf_dtree_l := (wf_dtree low high).
+Local Notation donesE := (@donesE low high).
+Local Notation dsizeE := (@dsizeE low high).
+
+Definition dins_leaf s b i :=
+  let s' := insert1 s b i in
+  if size s + 1 == high
+  then let n  := (size s') %/ 2 in
+       let sl := take n s' in
+       let sr := drop n s' in
+       Bnode Red (Bleaf _ sl) (size sl, count_mem true sl) (Bleaf _ sr)
+  else Bleaf _ s'.
+
+Definition lt_index i (d : nat * nat) := i < fst d.
+Definition right_index i (d : nat * nat) := i - fst d.
+
+Definition dins : dtree -> bool -> nat -> dtree :=
+  bins mkD dins_leaf lt_index right_index.
+Definition dinsert : dtree -> bool -> nat -> dtree :=
+  binsert mkD dins_leaf lt_index right_index.
+
+Lemma dins_leaf_is_redblack a b i : is_redblack (dins_leaf a b i) Black 0.
+Proof. rewrite /dins_leaf; by case: ifP. Qed.
+
+(* Red-blackness invariant *)
+Lemma dinsert_is_redblack B b i n :
+  is_redblack B Red n ->
+  is_redblack (dinsert B b i) Red (n + is_red (dins B b i)).
+Proof. apply /binsert_is_redblack /dins_leaf_is_redblack. Qed.
+
+(* Correctness of balance *)
+
+Lemma dflatten_node c l d r :
+  dflatten (Bnode c l d r) = dflatten l ++ dflatten r.
+Proof. by []. Qed.
+
+Lemma balanceE c l r : dflatten (balance c l r) = dflatten l ++ dflatten r.
+Proof.
+  rewrite /balance. case: c. exact: dflatten_node.
+  case: l => [[[[] lll llD llr|llA] lD [[] lrl lrD lrr|lrA]|ll lD lr]|lA] /=;
+  case: r => [[[[] rll rlD rlr|rlA] rD [[] rrl rrD rrr|rrA]|rl rD rr]|rA] /=;
+    try done; by rewrite !catA.
+Qed.
+
+Lemma balanceLE c l r : dflatten (balanceL c l r) = dflatten l ++ dflatten r.
+Proof.
+  rewrite /balanceL. case: c. exact: dflatten_node.
+  case: l => [[[[] lll llD llr|llA] lD [[] lrl lrD lrr|lrA]|ll lD lr]|lA] //=;
+    by rewrite !catA.
+Qed.
+
+Lemma balanceRE c l r : dflatten (balanceR c l r) = dflatten l ++ dflatten r.
+Proof.
+  rewrite /balanceR. case: c. exact: dflatten_node.
+  case: r => [[[[] rll rlD rlr|rlA] rD [[] rrl rrD rrr|rrA]|rl rD rr]|rA] //=;
+    by rewrite !catA.
+Qed.
+
+(* Well-foundedness lemmas
+ * Show that dinsert always returns a well-founded tree
+ *)
+
+Lemma balanceL_wf c (l r : dtree) :
+  wf_dtree_l l -> wf_dtree_l r -> wf_dtree_l (balanceL c l r).
+Proof.
+  case: c => /= wfl wfr.
+    by rewrite wfl wfr !(dsizeE,donesE,eqxx).
+  case: l wfl => [[[[] ? [??] ?|?] [??] [[] ? [??] ?|?] | ? [??] ?]|?] /=;
+    rewrite wfr; repeat decompose_rewrite;
+    by rewrite ?(dsizeE,donesE,size_cat,count_cat,eqxx).
+Qed.
+
+Lemma balanceR_wf c (l r : dtree) :
+  wf_dtree_l l -> wf_dtree_l r -> wf_dtree_l (balanceR c l r).
+Proof.
+  case: c => /= wfl wfr.
+    by rewrite wfl wfr ?(dsizeE,donesE,eqxx).
+  case: r wfr => [[[[] ? [??] ?|?] [??] [[] ? [??] ?|?] | ? [??] ?] | ?] /=;
+    rewrite wfl; repeat decompose_rewrite;
+    by rewrite ?(dsizeE,donesE,size_cat,count_cat,eqxx).
+Qed.
+
+Definition wf_dtree' t :=
+  if t is Bleaf s then size s < high else wf_dtree_l t.
+
+Lemma wf_dtree_dtree' t : wf_dtree_l t -> wf_dtree' t.
+Proof. by case: t => //= s /andP[_ ->]. Qed.
+
+Lemma wf_dtree'_dtree t : wf_dtree' t -> wf_dtree 0 high t.
+Proof.
+  elim: t => //= c l IHl [n o] r IHr; repeat decompose_rewrite => /=.
+  by rewrite !(IHl,IHr,wf_dtree_dtree').
+Qed.
+
+Lemma wf_dtree'_node c l d r :
+  wf_dtree' (Bnode c l d r) = wf_dtree low high (Bnode c l d r). 
+Proof. by []. Qed.
+
+Lemma leq_half n : n./2 <= n.
+Proof. by rewrite -{2}(odd_double_half n) -addnn addnA leq_addl. Qed.
+
+Lemma dins_leaf_wf s b i : size s < high -> wf_dtree' (dins_leaf s b i).
+Proof.
+  move=> Hs.
+  rewrite /dins_leaf addn1 divn2.
+  case: ifP => Hsize /=.
+    rewrite ?(eqxx,size_insert1,(eqP Hsize),size_drop,size_takel,leq_half) //.
+    have:= half_leq Hlow; rewrite doubleK => Hlow'.
+    set hhigh := high./2.
+    rewrite Hlow' -(odd_double_half high) -addnn addnA addnK.
+    have Hup : 0 < odd high + high./2.
       by rewrite -addn1 leq_add // (half_leq Hhigh).
-    move: Hs.
-    by rewrite size_insert1 leq_eqVlt Hsize /= => ->.
-  Qed.
+    rewrite -add1n leq_add // (leq_trans Hlow' (leq_addl _ _)).
+    by rewrite -addn1 leq_add // (half_leq Hhigh).
+  move: Hs.
+  by rewrite size_insert1 leq_eqVlt Hsize /= => ->.
+Qed.
 
-  Lemma dins_wf (B : dtree) b i :
-    wf_dtree low high B -> wf_dtree low high (dins B b i).
-  Proof.
-    move => wf;  move: B wf b i.
-    apply: dtree_ind =>
-           [c l r num ones -> -> [wfl wfr] IHl IHr b i | s Hs b i] /=.
-      case: ifP => Hi. by apply: balanceL_wf.
-      by apply: balanceR_wf.
-    have/andP[Hs1 Hs2]:= Hs.
-    have:= dins_leaf_wf b i Hs2.
-    case Hins: dins_leaf => [//|s'] /= ->.
-    move: Hins; rewrite /dins_leaf.
-    case: ifP => // _ [] <-.
-    by rewrite size_insert1 (leq_trans Hs1).
-  Qed.
+Lemma dins_wf (B : dtree) b i :
+  wf_dtree low high B -> wf_dtree low high (dins B b i).
+Proof.
+  move => wf;  move: B wf b i.
+  apply: dtree_ind =>
+         [c l r num ones -> -> [wfl wfr] IHl IHr b i | s Hs b i] /=.
+    case: ifP => Hi. by apply: balanceL_wf.
+    by apply: balanceR_wf.
+  have/andP[Hs1 Hs2]:= Hs.
+  have:= dins_leaf_wf b i Hs2.
+  case Hins: dins_leaf => [//|s'] /= ->.
+  move: Hins; rewrite /dins_leaf.
+  case: ifP => // _ [] <-.
+  by rewrite size_insert1 (leq_trans Hs1).
+Qed.
 
-  Lemma recolor_node_wf c c' d (l r : dtree) :
-    wf_dtree' (Bnode c l d r) -> wf_dtree' (Bnode c' l d r).
-  Proof. by []. Qed.
+Lemma recolor_node_wf c c' d (l r : dtree) :
+  wf_dtree' (Bnode c l d r) -> wf_dtree' (Bnode c' l d r).
+Proof. by []. Qed.
 
-  Definition is_leaf (t : dtree) := if t is Bleaf _ then true else false.
+Definition is_leaf (t : dtree) := if t is Bleaf _ then true else false.
 
-  Lemma dins_leaf_leaf t b i : is_leaf (dins t b i) ==> is_leaf t.
-  Proof.
-    apply/implyP.
-    case: t => //= c l [n o] r.
-    case: ifP => _ /=; rewrite /balanceL /balanceR; case: c => //=;
-     by case: dins => //= -[] // [[] ? ? ?|?] [n' o'] [[] ? ? ?|?].
-  Qed.
+Lemma dins_leaf_leaf t b i : is_leaf (dins t b i) ==> is_leaf t.
+Proof.
+  apply/implyP.
+  case: t => //= c l [n o] r.
+  case: ifP => _ /=; rewrite /balanceL /balanceR; case: c => //=;
+    by case: dins => //= -[] // [[] ? ? ?|?] [n' o'] [[] ? ? ?|?].
+Qed.
 
-  Lemma dinsert_wf (B : dtree) b i :
-    wf_dtree' B -> wf_dtree' (dinsert B b i).
-  Proof.
-    rewrite /dinsert => wf.
-    have:= @dins_leaf_leaf B b i.
-    case Hins: (dins B b i) => [c' l' [? ?] r' | s'] Hlf.
-      apply (@recolor_node_wf c').
-      case: B wf Hins {Hlf} => [c l [num ones] r | s] wf Hins.
-        apply wf_dtree_dtree'.
-        by rewrite -Hins dins_wf.
-      rewrite -Hins /=.
-      by apply dins_leaf_wf.
-    case: B wf Hins Hlf => //= s Hs Hins _.
-    move: (dins_leaf_wf b i Hs) => /=.
-    by rewrite Hins.
-  Qed.
+Lemma dinsert_wf (B : dtree) b i :
+  wf_dtree' B -> wf_dtree' (dinsert B b i).
+Proof.
+  rewrite /dinsert /binsert -/dins => wf.
+  have:= @dins_leaf_leaf B b i.
+  case Hins: (dins B b i) => [c' l' [? ?] r' | s'] Hlf.
+    apply (@recolor_node_wf c').
+    case: B wf Hins {Hlf} => [c l [num ones] r | s] wf Hins.
+      apply wf_dtree_dtree'.
+      by rewrite -Hins dins_wf.
+    rewrite -Hins /=.
+    by apply dins_leaf_wf.
+  case: B wf Hins Hlf => //= s Hs Hins b'.
+  move: (dins_leaf_wf b i Hs) => /=.
+  by rewrite Hins.
+Qed.
 
-  Definition dinsert_wf0 B b i wf := wf_dtree'_dtree (@dinsert_wf B b i wf).
+Definition dinsert_wf0 B b i wf := wf_dtree'_dtree (@dinsert_wf B b i wf).
 
-  Lemma dins_leafE s b i :
-    size s < high -> dflatten (dins_leaf s b i) = insert1 s b i.
-  Proof.
-    rewrite /dins /dins_leaf. case: ifP => Hi Hs //.
-    by rewrite dflatten_node /dflatten cat_take_drop.
-  Qed.
+(* Correctness of dinsert *)
 
-  Lemma dinsE (B : dtree) b i :
-    wf_dtree low high B -> dflatten (dins B b i) = insert1 (dflatten B) b i.
-  Proof.
-    move => wf; move: B wf b i. apply: dtree_ind => //.
-    + move => c l r num ones Hnum Hones _ IHl IHr /= b i.
-      case: ifPn => ?.
-      - by rewrite balanceLE IHl /insert1 insert_catL -?Hnum.
-      - by rewrite balanceRE IHr /insert1 insert_catR -?Hnum // leqNgt.
-    + move => s /andP [_] Hs b i /=.
-      by rewrite dins_leafE.
-  Qed.
+Lemma dins_leafE s b i :
+  size s < high -> dflatten (dins_leaf s b i) = insert1 s b i.
+Proof.
+  rewrite /dins /dins_leaf. case: ifP => Hi Hs //.
+  by rewrite dflatten_node /dflatten cat_take_drop.
+Qed.
 
-  Lemma dinsertE (B : dtree) b i :
-    wf_dtree' B -> dflatten (dinsert B b i) = insert1 (dflatten B) b i.
-  Proof.
-    case: B => [c l d r | s] wf.
-      rewrite /dinsert -(dinsE b i) //; by case: dins.
-    rewrite /dinsert /dins -dins_leafE; by case: dins_leaf.
-  Qed.
+Lemma dinsE (B : dtree) b i :
+  wf_dtree_l B -> dflatten (dins B b i) = insert1 (dflatten B) b i.
+Proof.
+  move => wf; move: B wf b i. apply: dtree_ind => //.
+  + move => c l r num ones Hnum Hones _ IHl IHr /= b i.
+    case: ifPn => ?.
+     - by rewrite balanceLE IHl /insert1 insert_catL -?Hnum.
+     - by rewrite balanceRE IHr /insert1 insert_catR -?Hnum // leqNgt.
+  + move => s /andP [_] Hs b i /=.
+    by rewrite dins_leafE.
+Qed.
 
-  Lemma dinsert_rank (B : dtree) b i j :
-    wf_dtree' B -> drank (dinsert B b i) j =
-                   rank true j (insert1 (dflatten B) b i).
-  Proof.
-    move => wf; by rewrite -dinsertE // (@drankE 0 high) // dinsert_wf0.
-  Qed.
+Lemma dinsertE (B : dtree) b i :
+  wf_dtree' B -> dflatten (dinsert B b i) = insert1 (dflatten B) b i.
+Proof.
+  case: B => [c l d r | s] wf.
+    rewrite /dinsert -(dinsE b i) /binsert /dins //; by case: bins.
+  rewrite /dinsert /binsert /dins -dins_leafE /=; by case: dins_leaf.
+Qed.
 
-  Lemma dinsert_select1 (B : dtree) b i j : wf_dtree' B ->
-    dselect_1 (dinsert B b i) j = select true j (insert1 (dflatten B) b i).
-  Proof.
-    move => wf; by rewrite -dinsertE // (@dselect_1E 0 high) // dinsert_wf0.
-  Qed.
+Lemma dinsert_rank (B : dtree) b i j :
+  wf_dtree' B -> drank (dinsert B b i) j =
+                 rank true j (insert1 (dflatten B) b i).
+Proof.
+  move => wf; by rewrite -dinsertE // (@drankE 0 high) // dinsert_wf0.
+Qed.
 
-  Lemma dinsert_select0 (B : dtree) b i j : wf_dtree' B ->
-   dselect_0 (dinsert B b i) j = select false j (insert1 (dflatten B) b i).
-  Proof.
-    move => wf; by rewrite -dinsertE // (@dselect_0E 0 high) // dinsert_wf0.
-  Qed.
+Lemma dinsert_select1 (B : dtree) b i j : wf_dtree' B ->
+  dselect_1 (dinsert B b i) j = select true j (insert1 (dflatten B) b i).
+Proof.
+  move => wf; by rewrite -dinsertE // (@dselect_1E 0 high) // dinsert_wf0.
+Qed.
 
-  (*
-   * Following Appel (2011), pp. 6 - 8
-   *
-   * ctxt = "color context", or the color of
-   * the parent node
-   *
-   * bh = "black height", i.e. # of black nodes on the
-   * path from the root
-   *)
-  Fixpoint is_redblack (B : dtree) ctxt bh :=
-    match B with
-    | Bleaf _ => bh == 0
-    | Bnode c l _ r =>
-      match c, ctxt with
-      | Red, Red => false
-      | Red, Black => is_redblack l Red bh
-                      && is_redblack r Red bh
-      | Black, _ => (bh > 0) && is_redblack l Black (bh.-1) &&
-                             is_redblack r Black (bh.-1)
-      end
-    end.
+Lemma dinsert_select0 (B : dtree) b i j : wf_dtree' B ->
+ dselect_0 (dinsert B b i) j = select false j (insert1 (dflatten B) b i).
+Proof.
+  move => wf; by rewrite -dinsertE // (@dselect_0E 0 high) // dinsert_wf0.
+Qed.
 
-  Definition nearly_redblack (B : dtree) bh :=
-    match B with
-    | Bnode Red l _ r => is_redblack l Black bh && is_redblack r Black bh
-    | _ => is_redblack B Black bh
-    end.
-
-  Lemma is_redblack_Red_Black B n :
-    is_redblack B Red n -> is_redblack B Black n.
-  Proof. by case: B => /= [[]|]. Qed.
-
-  Lemma balanceL_Black_nearly_is_redblack l r n :
-    nearly_redblack l n -> is_redblack r Black n ->
-    is_redblack (balanceL Black l r) Black n.+1.
-  Proof.
-    case: l => [[[[] lll ? llr|?] ? [[] lrl ? lrr|?]|ll ? lr]|?] /=;
-      repeat decompose_rewrite => //;
-      by rewrite !is_redblack_Red_Black -?(eqP H1).
-  Qed.
-
-  Lemma balanceR_Black_nearly_is_redblack l r n :
-    nearly_redblack r n -> is_redblack l Black n ->
-    is_redblack (balanceR Black l r) Black n.+1.
-  Proof.
-    case: r => [[[[] rll ? rlr|?] ? [[] rrl ? rrr|?]|rl ? rr]|?] /=;
-      repeat decompose_rewrite => //;
-      by rewrite !is_redblack_Red_Black -?(eqP H1).
-  Qed.
-
-  Lemma is_redblack_nearly_redblack B c n :
-    is_redblack B c n -> nearly_redblack B n.
-  Proof.
-    case: B => /= -[]; case: c => // l p r /andP [Hl Hr].
-    by rewrite !is_redblack_Red_Black.
-  Qed.
-
-  Lemma dins_is_redblack (B : dtree) b i n :
-    (is_redblack B Black n -> nearly_redblack (dins B b i) n) /\
-    (is_redblack B Red n -> is_redblack (dins B b i) Black n).
-  Proof.
-    elim: B i n => [c l IHl [num ones] r IHr | a] i n;
-      last by split => /=; rewrite /dins_leaf; case: ifP => //= _ ->.
-    have Hbk : is_redblack (Bnode Black l (num, ones) r) Black n ->
-               is_redblack (dins (Bnode Black l (num, ones) r) b i) Black n.
-      rewrite {3}[Black]lock /= -lock => /andP [/andP [/prednK <- Hl] Hr].
-      case: ifP => Hi.
-        rewrite balanceL_Black_nearly_is_redblack //; by apply IHl.
-      rewrite balanceR_Black_nearly_is_redblack //; by apply IHr.
-    split; case: c => //.
-    + move=> /= /andP [Hl Hr].
-      case: ifP => Hi /=; [move: Hr | move: Hl] => /is_redblack_Red_Black ->;
-        rewrite /= ?andbT; by [apply IHl | apply IHr].
-    + move/Hbk; by apply is_redblack_nearly_redblack.
-  Qed.
-
-  Lemma dinsert_is_redblack (B : dtree) b i n :
-    is_redblack B Red n -> exists n', is_redblack (dinsert B b i) Red n'.
-  Proof.
-    exists (if (dins B b i) is Bnode Red _ _ _ then n + 1 else n).
-    move/(proj2 (dins_is_redblack _ b i _)): H.
-    rewrite /dinsert addnC.
-    destruct dins => //=.
-    case: c => //= /andP [Hd1 Hd2].
-    by rewrite !is_redblack_Red_Black.
-  Qed.
-
-  Definition is_red D A (B : btree D A) :=
-    if B is Bnode Red _ _ _ then true else false.
-
-  Lemma dinsert_is_nearly_redblack' (B : dtree) b i n :
-    is_redblack B Red n ->
-    is_redblack (dinsert B b i) Red (n + is_red (dins B b i)).
-  Proof.
-    move/(proj2 (dins_is_redblack _ b i _)).
-    rewrite /dinsert addnC.
-    destruct dins => //=.
-    case: c => //= /andP [Hd1 Hd2].
-    by rewrite !is_redblack_Red_Black.
-  Qed.
-
-End insert_prop.
+End dinsert.
 
 Section set_clear.
 
@@ -793,409 +808,320 @@ Section set_clear.
 End set_clear.
 
 Section delete.
-  Variables low high : nat.
-  Hypothesis Hlow : low.*2 <= high.
-  Hypothesis Hlow1 : low >= 1.
-  Let Hhigh : 1 < high.
-  Proof. by rewrite (leq_trans _ Hlow) // (leq_double 1 low). Qed.
-  Local Notation wf_dtree' := (wf_dtree' low high).
-  Local Notation wf_dtree_l := (wf_dtree low high).
-  Local Notation donesE' := (@donesE low high).
-  Local Notation dsizeE' := (@dsizeE low high).
 
-  Inductive deleted_dtree: Type :=
-  | Stay : dtree -> deleted_dtree
-  | Down : dtree -> deleted_dtree.
+Variables D A : Type.
+Variable mkD : btree D A -> D.
 
-  Definition balanceL' col (l : deleted_dtree) (r : dtree) : deleted_dtree :=
-    match l with
-    | Stay l => Stay (rbnode col l r)
-    | Down l =>
-      match col,r with
-      | _, Bnode Black (Bnode Red rll _ rlr) _ rr =>
-        Stay (rbnode col (bnode l rll) (bnode rlr rr))
-      | Red, Bnode Black (Bleaf _ as rl) _ rr
-      | Red, Bnode Black (Bnode Black _ _ _ as rl) _ rr =>
-        Stay (bnode (rnode l rl) rr)
-      | Black,Bnode Red (Bnode Black (Bnode Black _ _ _ as rll) _ rlr) _ rr
-      | Black,Bnode Red (Bnode Black (Bleaf _ as rll) _ rlr) _ rr =>
-        Stay (bnode (bnode (rnode l rll) rlr) rr)
-      | Black,Bnode Red (Bnode Black (Bnode Red rlll _ rllr) _ rlr) _ rr =>
-        Stay (bnode (bnode l rlll) (rnode (bnode rllr rlr) rr))
-      | Black,Bnode Black (Bleaf _ as rl) _ rr 
-      | Black,Bnode Black (Bnode Black _ _ _ as rl) _ rr =>
-        Down (bnode (rnode l rl) rr)
-        (* absurd case *)
-      | _,_ => Stay (rbnode col l r)
-      end
-    end.
+Definition rbnode c l r := Bnode c l (mkD l) r.
+Definition bnode l r := Bnode Black l (mkD l) r.
+Definition rnode l r := Bnode Red l (mkD l) r.
+Local Notation leaf a := (Bleaf _ a : btree D A).
+
+Inductive deleted_btree: Type :=
+| Stay : btree D A -> deleted_btree
+| Down : btree D A -> deleted_btree.
+
+Definition balanceL' col (l : deleted_btree) r : deleted_btree :=
+  match l with
+  | Stay l => Stay (rbnode col l r)
+  | Down l =>
+    match col,r with
+    | _, Bnode Black (Bnode Red rll _ rlr) _ rr =>
+      Stay (rbnode col (bnode l rll) (bnode rlr rr))
+    | Red, Bnode Black (Bleaf _ as rl) _ rr
+    | Red, Bnode Black (Bnode Black _ _ _ as rl) _ rr =>
+      Stay (bnode (rnode l rl) rr)
+    | Black,Bnode Red (Bnode Black (Bnode Black _ _ _ as rll) _ rlr) _ rr
+    | Black,Bnode Red (Bnode Black (Bleaf _ as rll) _ rlr) _ rr =>
+      Stay (bnode (bnode (rnode l rll) rlr) rr)
+    | Black,Bnode Red (Bnode Black (Bnode Red rlll _ rllr) _ rlr) _ rr =>
+      Stay (bnode (bnode l rlll) (rnode (bnode rllr rlr) rr))
+    | Black,Bnode Black (Bleaf _ as rl) _ rr
+    | Black,Bnode Black (Bnode Black _ _ _ as rl) _ rr =>
+      Down (bnode (rnode l rl) rr)
+    | _,_ => Stay (rbnode col l r)
+    end
+  end.
   
-  Definition balanceR' col (l : dtree) (r : deleted_dtree) : deleted_dtree :=
-    match r with
-    | Stay r => Stay (rbnode col l r)
-    | Down r =>
-      match col,l with
-      | _, Bnode Black ll _ (Bnode Red lrl _ lrr) =>
-        Stay (rbnode col (bnode ll lrl) (bnode lrr r))
-      | Red,Bnode Black ll _ (Bleaf _ as lr)
-      | Red,Bnode Black ll _ (Bnode Black _ _ _ as lr) =>
-        Stay (bnode ll (rnode lr r))
-      | Black,Bnode Red ll _ (Bnode Black lrl _ (Bnode Black _ _ _ as lrr))
-      | Black,Bnode Red ll _ (Bnode Black lrl _ (Bleaf _ as lrr)) =>
-        Stay (bnode ll (bnode lrl (rnode lrr r)))
-      | Black,Bnode Red ll _ (Bnode Black lrl _ (Bnode Red lrrl _ lrrr)) =>
-        Stay (bnode (rnode ll (bnode lrl lrrl)) (bnode lrrr r))
-      | Black,Bnode Black ll _ (Bleaf _ as lr)
-      | Black,Bnode Black ll _ (Bnode Black _ _ _ as lr) =>
-        Down (bnode ll (rnode lr r))
-        (* absurd case *)
-      | _,_ => Stay (rbnode col l r)
-      end
-    end.
+Definition balanceR' col l (r : deleted_btree) : deleted_btree :=
+  match r with
+  | Stay r => Stay (rbnode col l r)
+  | Down r =>
+    match col,l with
+    | _, Bnode Black ll _ (Bnode Red lrl _ lrr) =>
+      Stay (rbnode col (bnode ll lrl) (bnode lrr r))
+    | Red,Bnode Black ll _ (Bleaf _ as lr)
+    | Red,Bnode Black ll _ (Bnode Black _ _ _ as lr) =>
+      Stay (bnode ll (rnode lr r))
+    | Black,Bnode Red ll _ (Bnode Black lrl _ (Bnode Black _ _ _ as lrr))
+    | Black,Bnode Red ll _ (Bnode Black lrl _ (Bleaf _ as lrr)) =>
+      Stay (bnode ll (bnode lrl (rnode lrr r)))
+    | Black,Bnode Red ll _ (Bnode Black lrl _ (Bnode Red lrrl _ lrrr)) =>
+      Stay (bnode (rnode ll (bnode lrl lrrl)) (bnode lrrr r))
+    | Black,Bnode Black ll _ (Bleaf _ as lr)
+    | Black,Bnode Black ll _ (Bnode Black _ _ _ as lr) =>
+      Down (bnode ll (rnode lr r))
+    | _,_ => Stay (rbnode col l r)
+    end
+  end.
 
-  Definition delete_leaves p l r (i : nat) : deleted_dtree :=
-    if i < size l
-    then match low == size l, low == size r with
-         | true,true =>
-           Down (leaf ((rcons (delete l i) (access r 0)) ++ (delete r 0)))
-         | true,false => 
-           Stay (rbnode p (leaf (rcons (delete l i) (access r 0))) (leaf (delete r 0)))
-         | false,_ => 
-           Stay (rbnode p (leaf (delete l i)) (leaf r))
-         end
-    else match low == size l, low == size r with
-         | true,true =>
-           Down (leaf (l ++ (delete r (i - (size l)))))
-         | false,true => 
-           Stay (rbnode p (leaf (delete l (size l).-1)) (leaf ((access l (size l).-1) :: (delete r (i - size l)))))
-         | _,false => 
-           Stay (rbnode p (leaf l) (leaf (delete r (i - (size l)))))
-         end.
+Variable lt_index : nat -> D -> bool.
+Variable right_index : nat -> D -> nat.
+Variable delete_leaf : A -> nat -> A.
+Variable delete_from_leaves : color -> A -> A -> nat -> deleted_btree.
 
-  Fixpoint height_of_dtree (B : dtree) :=
-    match B with
-    | Bnode Black l _ r => (maxn (height_of_dtree l) (height_of_dtree r)).+2
-    | Bnode Red l _ r => (maxn (height_of_dtree l) (height_of_dtree r)).+1
-    | Bleaf _ => 0
-    end.
+Fixpoint bdel B (i : nat) { struct B } : deleted_btree :=
+  match B with
+  | Bnode c (Bleaf l) d (Bleaf r) => delete_from_leaves c l r i
+  | Bnode Black (Bnode Red (Bleaf ll) ld (Bleaf lr) as l) d (Bleaf r) =>
+    if lt_index i d
+    then balanceL' Black (bdel l i) (Bleaf _ r)
+    else balanceR' Black (Bleaf _ ll)
+                   (delete_from_leaves Red lr r (right_index i ld))
+  | Bnode Black (Bleaf l) ld (Bnode Red (Bleaf rl) rd (Bleaf rr) as r) =>
+    if lt_index (right_index i ld) rd
+    then balanceL' Black (delete_from_leaves Red l rl i) (Bleaf _ rr)
+    else balanceR' Black (Bleaf _ l) (bdel r (right_index i ld))
+  | Bnode c l d r => 
+    if lt_index i d
+    then balanceL' c (bdel l i) r
+    else balanceR' c l (bdel r (right_index i d))
+  | Bleaf x =>  Stay (leaf (delete_leaf x i))
+  end.
 
-  Lemma hc_pcl {l r c s n} :
-    height_of_dtree l < height_of_dtree (Bnode c l (s, n) r).
-  Proof.
-    case c; rewrite /= -!maxnSS leq_max ltnS;
-    [ rewrite leqnn // | rewrite ltnW // ].
-  Qed.
+Definition is_nearly_redblack' tr c bh :=
+  match tr with
+  | Stay tr => is_redblack tr c bh
+  | Down tr => is_redblack tr Red bh.-1
+  end.
 
-  Lemma hc_pcr {l r c s n} :
-    height_of_dtree r < height_of_dtree (Bnode c l (s, n) r).
-  Proof.
-    case c; rewrite /= -!maxnSS leq_max ltnS;
-    [ rewrite leqnn orbT // | apply/orP; right; rewrite ltnW // ]. 
-  Qed.
-
-  Lemma hc_pcl' {lr ll r s p n} :
-    height_of_dtree (rnode lr r) < height_of_dtree (Bnode Black (Bnode Red ll p lr) (s, n) r).
-  Proof.
-    rewrite /= -!maxnSS -maxnA !leq_max !/maxn; case: ifP => H;
-    [ rewrite ltnSn !orbT // | rewrite [ _.+1 < (_ lr).+3]ltnW // orbT // ]. 
-  Qed.
-
-  Lemma hc_pcr' {l rl rr s n p} :
-    height_of_dtree (rnode l rl) < height_of_dtree (Bnode Black l (s, n) (Bnode Red rl p rr)).
-  Proof.
-    rewrite /= -!maxnSS maxnA !leq_max !/maxn; case: ifP => H;
-   [ rewrite [ _.+1 < (_ rl).+3]ltnW // orbT // | rewrite ltnSn // ]. 
-  Qed.
+Hypothesis Hdelete_from_leaves : forall c l d r i c' n,
+  is_redblack (Bnode c (Bleaf D l) d (Bleaf D r)) c' n ->
+  is_nearly_redblack' (delete_from_leaves c l r i) c' n.
   
-  Lemma hc_pcr'' {ll lr rl rr lc l' dr}:
-    height_of_dtree (rnode (rbnode lc ll lr) (bnode rl rr)) <
-    height_of_dtree (bnode (rnode (leaf l') (rbnode lc ll lr)) (Bnode Black rl dr rr)).
-  Proof.
-    move: lc => /= []; rewrite max0n !maxnSS /= /leq !subSS subn_eq0;
-    rewrite /= -!maxnSS maxnA !leq_max !/maxn;
-    repeat case: ifP;
-    try rewrite leqnn //=;
-    try rewrite leqnSn //=;
-    by (intros; rewrite !orbT).
-  Qed.
-
-  Function ddel (B : dtree) (i : nat) { measure height_of_dtree B } : deleted_dtree :=
-    match B with
-    | Bnode Black (Bleaf l) (s,o) (Bleaf r) => delete_leaves Black l r i
-    | Bnode Red (Bleaf l) (s,o) (Bleaf r) => delete_leaves Red l r i
-    | Bnode Black (Bnode Red (Bleaf ll) (ls,_) (Bleaf lr)) (s,_) (Bleaf r) => 
-      if i < s
-      then balanceL' Black (delete_leaves Red ll lr i) (Bleaf _ r)
-      else balanceR' Black (Bleaf _ ll) (delete_leaves Red lr r (i - ls))
-    | Bnode Black (Bleaf l) (ls,_) (Bnode Red (Bleaf rl) (rs,_) (Bleaf rr)) => 
-      if i < ls + rs
-      then balanceL' Black (delete_leaves Red l rl i) (Bleaf _ rr)
-      else balanceR' Black (Bleaf _ l) (delete_leaves Red rl rr (i - ls))
-    | Bnode Black (Bnode Black ll (ls,lo) lr) (s,_) (Bnode Red rl (rs,ro) rr) =>
-      let l := Bnode Black ll (ls,lo) lr in
-      let r := Bnode Red rl (rs,ro) rr in
-      if i < s
-      then balanceL' Black (ddel (rnode l rl) i) rr
-      else balanceR' Black l (ddel r (i - s))
-    | Bnode Black (Bnode Red ll (ls,lo) lr) (s,_) (Bnode Black rl (rs,ro) rr) =>
-      let l := Bnode Red ll (ls,lo) lr in
-      let r := Bnode Black rl (rs,ro) rr in
-      if i < s
-      then balanceL' Black (ddel l i) r
-      else balanceR' Black ll (ddel (rnode lr r) (i - ls))
-    | Bnode c l (s,_) r => 
-      if i < s
-      then balanceL' c (ddel l i) r
-      else balanceR' c l (ddel r (i - s))
-    (* absurd case *)
-    | Bleaf x =>  Stay (leaf (delete x i))
-    end.
-
-  all: intros; subst B; apply/leP; 
-  try (apply/eqP; rewrite /= subSS; apply/eqP; try (by apply leq_maxl); by apply leq_maxr); 
-  try (apply hc_pcl); try (apply hc_pcr).
-  apply hc_pcl'.
-  apply hc_pcr''.
-  apply hc_pcr'.
-  Defined.
-
-  Lemma ddel0E s o l r i :
-    ddel (Bnode Red (Bleaf (nat * nat) l) (s,o) (Bleaf (nat * nat) r)) i = delete_leaves Red l r i.
-  Proof.
-    move Heq : (Bnode Red _ _ _) => B; 
-    functional induction (ddel B i) => //=; 
-    move: Heq => /=; try (by move => Heq; case: Heq y => <- <- ? ? <-; case c => //);
-    by case => -> ? ? ->. 
-  Qed.
-
-  Definition dflattenn tr :=
-    match tr with
-    | Stay t => dflatten t
-    | Down t => dflatten t
-    end.
-
-  Lemma balanceL'E c l r : dflattenn (balanceL' c l r) = dflattenn l ++ dflatten r.
-  Proof. 
-    move: l => [] ?; case c; case r => [] [] // [] //= [] [] [] /=; 
-    intros; rewrite //= -!catA //= -!catA //. 
-  Qed.
-
-  Lemma balanceR'E c l r : dflattenn (balanceR' c l r) = dflatten l ++ dflattenn r.
-  Proof.
-    move: r => [] ?; case c; case l => //= [c'] ? ? [c''|]; 
-    try case c'; try case c''; try (intros; rewrite //= -!catA //= -!catA //=);
-    move => ? ? [] x; first case x; intros; rewrite //= -!catA //= -!catA //=.
-  Qed.
-
-  Lemma delete_cat {arr arr' : seq bool} {i} :
-    delete (arr ++ arr') i = (if i < size arr then delete arr i ++ arr' else arr ++ delete arr' (i - (size arr))).
-  Proof.
-    rewrite /delete take_cat -catA drop_cat.
-    case: ifP => H1; case: ifP => // H2; try (move: (ltnW H2); by rewrite H1).
-     have H3 : i.+1 = size arr; first by apply/eqP; rewrite eqn_leq H1 leqNgt H2.
-     by rewrite H3 subnn drop0 drop_oversize.
-    by rewrite catA subSn // leqNgt H1.
-  Qed.
-
-  Lemma delete_leavesE c l r i :
-    low <= size l < high -> low <= size r < high ->
-    dflattenn (delete_leaves c l r i) = delete (l ++ r) i.
-  Proof.
-    rewrite /delete_leaves delete_cat.
-    case: ifP; case: ifP => //; case: ifP => //;
-      try rewrite /delete /= take0 drop1 cat0s cat_rcons -!catA.
-        case r => //= /eqP -> /eqP <-; by rewrite ltn0.
-      case r => //= Hlow0 _ _ _ /andP []; by rewrite leqn0 Hlow0.
-    move/eqP => -> /= Hnl Hi /andP [Hl Hl'] Hr'.
-    have Hl0 : 0 < size l by move: Hl; rewrite leq_eqVlt Hnl /=; case: (size l).
-    rewrite /delete /= /access drop_oversize ?prednK //.
-    by rewrite cats0 -cat_rcons -take_nth prednK // take_oversize.
-  Qed.
-
-Let summand_leq a b c : a + b <= c -> a <= c.
-Proof. by apply: leq_trans; rewrite leq_addr. Qed.
-  
-  Lemma ddelE (B : dtree) i :
-    wf_dtree_l B -> dflattenn (ddel B i) = delete (dflatten B) i.
-  Proof.
-    functional induction (ddel B i)
-      => //= /andP [/eqP Hs] /andP [_] /andP [wfl wfr].
-    + by rewrite /= /ddel delete_leavesE.
-    + by rewrite /= /ddel delete_leavesE.
-    + rewrite balanceL'E delete_leavesE //;
-      move: wfl wfr; repeat decompose_rewrite => /=; try by [].
-      rewrite !delete_cat //= !size_cat //=.
-      repeat case:ifP => //=;
-      move:Hs; rewrite size_cat => <-; rewrite e0 //.
-      
-    + rewrite balanceR'E delete_leavesE //;
-      try move: wfl wfr; repeat decompose_rewrite => //=.
-      rewrite !delete_cat //= !size_cat //=.
-      move:y Hs; case: ifP => //; rewrite size_cat=>y _ Hs.
-      move:(Hs)(y)=>->->.
-      case: ifP.
-       rewrite /leq -subSn;
-       last (move:y;rewrite ltnNge Hs; move/negPn; apply summand_leq);
-       rewrite -subnDA subn_eq0 -Hs y //.
-      rewrite subnDA !catA //=.
-      
-    + rewrite balanceL'E delete_leavesE //;
-      move: wfl wfr; repeat decompose_rewrite => /=; try by [].
-      rewrite !delete_cat //=.
-      repeat case: ifP; try by rewrite !catA.
-      move:e0;move/eqP:H1=>->;move:Hs=>-> X Y Z.
-      move:Z; rewrite ltnNge /=; move/negPn=>?.
-      move:X Y; rewrite /leq.
-      rewrite -subSn // !subnDA => -> //.
-      
-    + rewrite balanceR'E delete_leavesE //;
-      try move: wfl wfr; repeat decompose_rewrite => //=.
-      rewrite !delete_cat //=.
-      move:y;case: ifP => //;rewrite ltnNge;move/negPn=>y _.
-      move/eqP:(H1) (Hs) y =>->-> y.
-      repeat case: ifP;
-      try by rewrite !catA;
-      try by rewrite ltnNge (summand_leq y).
-      
-    + rewrite balanceL'E IHd; last first.
-        move: wfl wfr; repeat decompose_rewrite => /=.
-        by rewrite size_cat !dsizeE' // count_cat !donesE' // !eqxx.
-      by rewrite !catA [RHS]delete_cat size_cat -Hs ltn_addr.
-      
-    + case: ifP y => // e0 _.
-      by rewrite balanceR'E delete_cat -Hs e0 IHd.
-    + by rewrite balanceL'E delete_cat -Hs e0 IHd.
-    + rewrite balanceR'E IHd; last first.
-        move: wfl wfr; repeat decompose_rewrite => /=.
-        by rewrite dsizeE' // donesE' // !eqxx.
-      rewrite -!catA // delete_cat.
-      case: ifP => H.
-        by case: ifP y => //; rewrite Hs size_cat ltn_addr.
-      by move: wfl; repeat decompose_rewrite => //.
-    + by rewrite balanceL'E delete_cat -Hs e0 IHd.
-    + case: ifP y0 => // e0 _.
-      by rewrite balanceR'E delete_cat -Hs e0 IHd.
-  Qed.
-
-  Definition is_nearly_redblack' tr c bh :=
-    match tr with
-    | Stay tr => is_redblack tr c bh
-    | Down tr => is_redblack tr Red bh.-1
-    end.
-  
-  Lemma is_nearly_redblack'_Red_Black B n :
-    is_nearly_redblack' B Red n -> is_nearly_redblack' B Black n.
-  Proof. case: B => [[]|] //= [] //. Qed.
+Lemma is_nearly_redblack'_Red_Black B n :
+  is_nearly_redblack' B Red n -> is_nearly_redblack' B Black n.
+Proof. case: B => [[]|] //= [] //. Qed.
     
-  Lemma balanceL'_Black_nearly_is_redblack l r n c :
-    0 < n -> is_nearly_redblack' l Black n.-1 -> is_redblack r Black n.-1 ->
-    is_nearly_redblack' (balanceL' Black l r) c n.
-  Proof.
-    case: l => [l /= -> -> -> // | l Hn okl okr].
-    case: c n r l okr okl Hn => [] [//|n]
-      [[[[] [[] rlll ? rllr|?] ? rlr|?] ? rr| [[] rll ? rlr| ?] ? rr]|?] l //=;
-    repeat decompose_rewrite => //; by rewrite !is_redblack_Red_Black.
-  Qed.
-  
-  Lemma balanceL'_Red_nearly_is_redblack l r n :
-    is_nearly_redblack' l Red n -> is_redblack r Red n ->
-    is_nearly_redblack' (balanceL' Red l r) Black n.
-  Proof.
-    case: l => [l /= -> -> // | l okl okr].
-    case: r l okr okl => [ [//|] [[] rll ? rlr| ?] ? rr | ?] l /=;
-    repeat decompose_rewrite => //; by rewrite !is_redblack_Red_Black.
-  Qed.
-    
-  Lemma balanceR'_Black_nearly_is_redblack l r n c :
-    0 < n -> is_redblack l Black n.-1 -> is_nearly_redblack' r Black n.-1 ->
-    is_nearly_redblack' (balanceR' Black l r) c n.
-  Proof.
-    case: r => [r /= -> -> -> //| //].
-    case: c n l => [] [//|n] [[[[] lll ? llr|?] ?
-      [[] lrl ? [[] lrrl ? lrrr|?]|?]|ll ? [[] lrl ? lrr|?]]|?] /=;
-    repeat decompose_rewrite => //; by rewrite !is_redblack_Red_Black. 
-  Qed.
-  
-  Lemma balanceR'_Red_nearly_is_redblack l r n :
-    is_redblack l Red n -> is_nearly_redblack' r Red n ->
-    is_nearly_redblack' (balanceR' Red l r) Black n.
-  Proof.
-    case: r => [r /= -> -> //| //].
-    case: l => [ [//|] ll ? [[] lrl ? lrr|?] |?] r /=;
-    repeat decompose_rewrite => //; by rewrite !is_redblack_Red_Black. 
-  Qed.
-  
-Ltac decomp ok := move: ok => /=; repeat decompose_rewrite.
-Ltac solveL' IHd ok :=
-  rewrite balanceL'_Black_nearly_is_redblack // ?IHd //; decomp ok.
-Ltac solveR' IHd ok :=
-  rewrite balanceR'_Black_nearly_is_redblack // ?IHd //; decomp ok.
-Ltac splitL' t y IHd ok :=
-  case: t => [[] ? ? ?|?] // in y IHd ok *; try by solveL' IHd ok.
-Ltac splitR' t y IHd ok :=
-  case: t => [[] ? ? ?|?] // in y IHd ok *; try by solveR' IHd ok.
-Ltac decomp_ifP ok :=
-  repeat case: ifP => ?; decomp ok.
-
-Lemma ddel_is_nearly_redblack' B i n c :
-  0 < n -> is_redblack B c n -> is_nearly_redblack' (ddel B i) c n.
+Lemma balanceL'_Black_nearly_is_redblack l r n c :
+  0 < n -> is_nearly_redblack' l Black n.-1 -> is_redblack r Black n.-1 ->
+  is_nearly_redblack' (balanceL' Black l r) c n.
 Proof.
-move: n c; functional induction (ddel B i) => n c' H.
-+ rewrite /delete_leaves.
-  case: c' => /= ok; by decomp_ifP ok.
-+ rewrite /delete_leaves.
-  case: c' => /= ok; by decomp_ifP ok.
-+ rewrite /delete_leaves.
-  case: c' => /= ok; by decomp_ifP ok.
-+ rewrite /delete_leaves.
-  case: c' => /= ok; by decomp_ifP ok.
-+ rewrite /delete_leaves.
-  case: c' => /= ok; by decomp_ifP ok.
-+ rewrite /delete_leaves.
-  case: c' => /= ok; by decomp_ifP ok.
-+ move=> ok; solveL' IHd ok => //.
-  by apply is_redblack_Red_Black.
-+ move=> ok; by solveR' IHd ok.
-+ move=> ok; by solveL' IHd ok.
-+ move=> ok; solveR' IHd ok => //.
-  by apply is_redblack_Red_Black.
-+ move: c c' l r y IHd =>
-    [] [] // [[] ll [] ? ? lr |?] [[] // rl [] ? ? rr|?] //= y IHd;
-  first (by rewrite !andbF);
-  try (case/andP => C /eqP H'; case/andP: C; by rewrite H' ltnn /=);
-  move => ok;
-  first (by rewrite balanceL'_Red_nearly_is_redblack // ?IHd //; decomp ok);
-  splitL' ll y IHd ok;
-  splitL' lr y IHd ok;
-  try splitL' rl y IHd ok;
-  by rewrite ddel0E /delete_leaves; decomp_ifP ok.
-+ move: c c' l r y IHd =>
-    [] [] // [[] ll [] ? ? lr |?] [[] // rl [] ? ? rr|?] //= y IHd;
-  try (by rewrite !andbF);
-  try (case/andP => /eqP ->; by rewrite ltnn /=);
-  move => ok;
-  first (by rewrite balanceR'_Red_nearly_is_redblack // ?IHd //; decomp ok);
-  splitR' rl y IHd ok;
-  splitR' rr y IHd ok;
-  try splitR' lr y IHd ok;
-  by rewrite ddel0E /delete_leaves; decomp_ifP ok.
-+ by [].
+  case: l => [l /= -> -> -> // | l Hn okl okr].
+  case: c n r l okr okl Hn => [] [//|n]
+    [[[[] [[] rlll ? rllr|?] ? rlr|?] ? rr| [[] rll ? rlr| ?] ? rr]|?] l //=;
+  repeat decompose_rewrite; by rewrite // !is_redblack_Red_Black.
+Qed.
+  
+Lemma balanceL'_Red_nearly_is_redblack l r n :
+  is_nearly_redblack' l Red n -> is_redblack r Red n ->
+  is_nearly_redblack' (balanceL' Red l r) Black n.
+Proof.
+  case: l => [l /= -> -> // | l okl okr].
+  case: r l okr okl => [ [//|] [[] rll ? rlr| ?] ? rr | ?] l /=;
+  repeat decompose_rewrite; by rewrite // !is_redblack_Red_Black.
+Qed.
+    
+Lemma balanceR'_Black_nearly_is_redblack l r n c :
+  0 < n -> is_redblack l Black n.-1 -> is_nearly_redblack' r Black n.-1 ->
+  is_nearly_redblack' (balanceR' Black l r) c n.
+Proof.
+  case: r => [r /= -> -> -> //| //].
+  case: c n l => [] [//|n] [[[[] lll ? llr|?] ?
+    [[] lrl ? [[] lrrl ? lrrr|?]|?]|ll ? [[] lrl ? lrr|?]]|?] /=;
+  repeat decompose_rewrite; by rewrite // !is_redblack_Red_Black. 
+Qed.
+  
+Lemma balanceR'_Red_nearly_is_redblack l r n :
+  is_redblack l Red n -> is_nearly_redblack' r Red n ->
+  is_nearly_redblack' (balanceR' Red l r) Black n.
+Proof.
+  case: r => [r /= -> -> //| //].
+  case: l => [ [//|] ll ? [[] lrl ? lrr|?] |?] r /=;
+  repeat decompose_rewrite; by rewrite // !is_redblack_Red_Black. 
+Qed.
+  
+Ltac close_branch d H IHl IHr :=
+ rewrite /=;
+ try case:ifP=>?;
+ rewrite ?(balanceL'_Red_nearly_is_redblack,
+           balanceR'_Red_nearly_is_redblack,
+           balanceL'_Black_nearly_is_redblack,
+           balanceR'_Black_nearly_is_redblack,
+           IHl, IHr, Hdelete_from_leaves (d:=d));
+ decomp H.
+
+Lemma bdel_is_nearly_redblack' B i n c :
+  is_redblack B c n -> is_nearly_redblack' (bdel B i) c n.
+Proof.
+elim: B c i n => // c l IHl d r IHr p i n H //.
+time (case: p c l IHl H => [] []// [[]//[[]//???|?]?[[]//???|?]|?] IHl H;
+  try (by close_branch d H IHl IHr);
+  case: r IHr H => [[]//[[]//???|?]?[[]//???|?]|?] IHr H;
+  by close_branch d H IHl IHr).
 Qed.
 
-Definition identify_deleted_dtree B :=
+End delete.
+
+Section ddelete.
+
+Variables low high : nat.
+Hypothesis Hlow : low.*2 <= high.
+Hypothesis Hlow1 : low >= 1.
+Let Hhigh : 1 < high.
+Proof. by rewrite (leq_trans _ Hlow) // (leq_double 1 low). Qed.
+Local Notation wf_dtree' := (wf_dtree' low high).
+Local Notation wf_dtree_l := (wf_dtree low high).
+Local Notation donesE' := (@donesE low high).
+Local Notation dsizeE' := (@dsizeE low high).
+Local Notation leaf a := (Bleaf _ a : dtree).
+Local Notation rbnode := (rbnode mkD).
+Definition deleted_dtree := deleted_btree (nat * nat) (seq bool).
+Local Notation balanceL' c B b := (balanceL' mkD c B b : deleted_dtree).
+Local Notation balanceR' c B b := (balanceR' mkD c B b : deleted_dtree).
+
+Definition delete_from_leaves (p : color) l r (i : nat) : deleted_dtree :=
+  if i < size l
+  then match low == size l, low == size r with
+       | true,true =>
+         Down (leaf ((rcons (delete l i) (access r 0)) ++ (delete r 0)))
+       | true,false => 
+         Stay (rbnode p (leaf (rcons (delete l i) (access r 0)))
+                          (leaf (delete r 0)))
+       | false,_ => 
+         Stay (rbnode p (leaf (delete l i)) (leaf r))
+       end
+  else match low == size l, low == size r with
+       | true,true =>
+         Down (leaf (l ++ (delete r (i - (size l)))))
+       | false,true => 
+         Stay (rbnode p (leaf (delete l (size l).-1))
+                   (leaf (access l (size l).-1 :: delete r (i - size l))))
+       | _,false => 
+         Stay (rbnode p (leaf l) (leaf (delete r (i - size l))))
+       end.
+
+Lemma delete_from_leaves_nearly_redblack' c l d r i c' n :
+  is_redblack (Bnode c (leaf l) d (leaf r)) c' n ->
+  is_nearly_redblack' (delete_from_leaves c l r i) c' n.
+Proof.
+  rewrite /delete_from_leaves.
+  case: c c' => /= -[]; repeat case: ifP => ?; repeat decompose_rewrite => //=.
+Qed.
+
+Notation ddel := (bdel mkD lt_index right_index (@delete _) delete_from_leaves).
+
+(* Red-blackness invariant *)
+Lemma ddel_is_nearly_redblack' B i n c :
+  is_redblack B c n -> is_nearly_redblack' (ddel B i) c n.
+Proof. apply /bdel_is_nearly_redblack' /delete_from_leaves_nearly_redblack'. Qed.
+
+(* Correctness lemmas *)
+
+Lemma ddel0E s o l r i :
+  ddel (Bnode Red (leaf l) (s,o) (leaf r)) i = delete_from_leaves Red l r i.
+Proof.
+  move Heq : (Bnode Red _ _ _) => B.
+  by case: B Heq => [[]//???|?] <-.
+Qed.
+
+Definition dflattenn tr :=
+  match tr with
+  | Stay t => dflatten t
+  | Down t => dflatten t
+  end.
+
+Lemma balanceL'E c l r :
+  dflattenn (balanceL' c l r) = dflattenn l ++ dflatten r.
+Proof. 
+  move: l => [] ?; case c; case r => [] [] // [] //= [] [] [] /=; 
+  intros; rewrite //= -!catA //= -!catA //. 
+Qed.
+
+Lemma balanceR'E c l r :
+  dflattenn (balanceR' c l r) = dflatten l ++ dflattenn r.
+Proof.
+  move: r => [] ?; case c; case l => //= [c'] ? ? [c''|]; 
+  try case c'; try case c''; try (intros; rewrite //= -!catA //= -!catA //=);
+  move => ? ? [] x; first case x; intros; rewrite //= -!catA //= -!catA //=.
+Qed.
+
+Lemma delete_cat {arr arr' : seq bool} {i} :
+  delete (arr ++ arr') i =
+  if i < size arr then delete arr i ++ arr'
+                  else arr ++ delete arr' (i - size arr).
+Proof.
+  rewrite /delete take_cat -catA drop_cat.
+  case: ifP => H1; case: ifP => // H2; try (move: (ltnW H2); by rewrite H1).
+    have H3 : i.+1 = size arr; first by apply/eqP; rewrite eqn_leq H1 leqNgt H2.
+    by rewrite H3 subnn drop0 drop_oversize.
+  by rewrite catA subSn // leqNgt H1.
+Qed.
+
+Lemma delete_from_leavesE c l r i :
+  low <= size l < high -> low <= size r < high ->
+  dflattenn (delete_from_leaves c l r i) = delete (l ++ r) i.
+Proof.
+  rewrite /delete_from_leaves delete_cat.
+  case: ifP; case: ifP => //; case: ifP => //;
+    try rewrite /delete /= take0 drop1 cat0s cat_rcons -!catA.
+      case r => //= /eqP -> /eqP <-; by rewrite ltn0.
+    case r => //= Hlow0 _ _ _ /andP []; by rewrite leqn0 Hlow0.
+  move/eqP => -> /= Hnl Hi /andP [Hl Hl'] Hr'.
+  have Hl0 : 0 < size l by move: Hl; rewrite leq_eqVlt Hnl /=; case: (size l).
+  rewrite /delete /= /access drop_oversize ?prednK //.
+  by rewrite cats0 -cat_rcons -take_nth prednK // take_oversize.
+Qed.
+  
+Lemma ltn_subLR m n p : 0 < p -> (m - n < p) = (m < n + p).
+Proof. case: p => //= p; by rewrite addnS !ltnS leq_subLR. Qed.
+
+Lemma ddel_cat c l a b r i :
+  wf_dtree_l (Bnode c l (a, b) r) ->
+  dflattenn (ddel (Bnode c l (a, b) r) i) =
+  if i < a
+  then dflattenn (ddel l i) ++ dflatten r
+  else dflatten l ++ dflattenn (ddel r (i - a)).
+Proof.
+  rewrite /= /lt_index /right_index /=.
+  time (case: ifP => Hc; case: c l r =>
+      [] [[]// [??[??]?|?] [??] [??[??]?|?]|?]
+      [[] [??[??]?|?] [??] [??[??]?|?]|?] wfB //;
+    try case:ifP;
+    rewrite ?(balanceL'E, balanceR'E, delete_cat, delete_from_leavesE,
+              ltn_subLR, leq_trans Hlow1) //;
+    move:wfB Hc; rewrite ?size_cat;
+    do! (decompose_rewrite; try by rewrite ltn_addr) => //=).
+  all: by rewrite ?(subnDA, catA).
+Qed.
+
+Lemma ddelE (B : dtree) i :
+  wf_dtree_l B -> dflattenn (ddel B i) = delete (dflatten B) i.
+Proof.
+ elim:B i => [c l IHl [??] r IHr|B] i wfB.
+ rewrite delete_cat.
+ rewrite -IHl; last by decomp wfB.
+ rewrite -IHr; last by decomp wfB.
+ rewrite ddel_cat //; by decomp wfB.
+ by rewrite /=.
+Qed.
+
+(* Well-formedness *)
+
+Definition dtree_of_deleted_dtree (B : deleted_dtree) : dtree :=
   match B with
   | Stay b => b
   | Down b => b
   end.
 
-Coercion identify_deleted_dtree : deleted_dtree >-> dtree.
+Coercion dtree_of_deleted_dtree : deleted_dtree >-> dtree.
 
 Lemma balanceL'_wf (B: deleted_dtree) b c:
   wf_dtree_l B -> wf_dtree_l b -> wf_dtree_l (balanceL' c B b).
 Proof.
   case: B b => B b /= wfB wfb.
     by rewrite dsizeE' // donesE' // !eqxx wfB wfb.
-  move: c b wfb => [][[][[][[]?[]???|?][]???|?][]??[[]?[]???|?]|?] /=;
+  move: c b wfb => [][[][[][[]?[??]?|?][??]?|?][??][[]?[??]?|?]|?] /=;
    do !decompose_rewrite => //;
    by rewrite !(size_cat,count_cat,addnA,catA,dsizeE',donesE',eqxx,wfB).
 Qed.
@@ -1205,30 +1131,27 @@ Lemma balanceR'_wf (B: deleted_dtree) b c:
 Proof.
   case: B b => B b /= wfB wfb.
     by rewrite dsizeE' // donesE' // !eqxx wfB wfb.
-  move: c b wfb => [][[][[]?[]???|?][]??[[]?[]??[[]?[]???|?]|?]|?] /=;
+  move: c b wfb => [][[][[]?[??]?|?][??][[]?[??][[]?[??]?|?]|?]|?] /=;
    do! decompose_rewrite => //;
-   by rewrite ?(size_cat,count_cat,addnA,catA,dsizeE',donesE',eqxx,wfB).
+   by rewrite !(size_cat,count_cat,addnA,catA,dsizeE',donesE',eqxx,wfB).
 Qed.
 
 Lemma leq_predr (m n : nat) :
   (m == n) = false -> m <= n -> m <= n.-1.
 Proof. rewrite leq_eqVlt => -> /= lo; by rewrite -ltnS (ltn_predK lo). Qed.
 
-Lemma ltn_subLR m n p : 0 < p -> (m - n < p) = (m < n + p).
-Proof. case: p => //= p; by rewrite addnS !ltnS leq_subLR. Qed.
-
-Lemma delete_leaves_wf l r i c:
+Lemma delete_from_leaves_wf l r i c:
   i < size l + size r ->
   low <= size l < high ->
   low <= size r < high ->
-  wf_dtree_l (delete_leaves c l r i).
+  wf_dtree_l (delete_from_leaves c l r i).
 Proof.
-  move=>sc /andP [wll wlh] /andP [wrl wrh].
+  move=> sc /andP [wll wlh] /andP [wrl wrh].
   have szl: 0 < size l by apply (leq_trans Hlow1).
   have szr: 0 < size r by apply (leq_trans Hlow1).
   have szlp: (size l).-1 < size l by rewrite prednK // subnn.
   have szrp: (size r).-1 < size r by rewrite prednK // subnn.
-  rewrite /delete_leaves; do! case: ifP; move=>rc lc /=; try (move=> Hi);
+  rewrite /delete_from_leaves; do! case: ifP; move=>rc lc /=; try (move=> Hi);
   rewrite ?(size_cat,size_rcons,size_delete,eqxx) //=;
   rewrite ?(prednK,wll,wlh,wrl,wrh) // -?(eqP rc,eqP lc);
   try (by rewrite leq_addr (leq_trans _ Hlow)// -addnn ltn_add2l prednK);
@@ -1236,106 +1159,70 @@ Proof.
   by rewrite {1}(eqP lc) (eqP rc).
 Qed.
 
-Lemma dsize_gt0 (B: dtree) : wf_dtree_l B -> dsize B > 0.
+Lemma dsize_gt0 (B: dtree) : wf_dtree_l B -> size (dflatten B) > 0.
 Proof.
   move: B; apply: dtree_ind => [c l r num ones -> -> [wfl wfr] IHl IHr|s wf] /=.
-    by rewrite ltn_addr.
+    by rewrite size_cat ltn_addr.
   rewrite (leq_trans Hlow1); by decomp wf.
-Qed.
-  
-Lemma stay_wfL ll lr r i s:
-  s == size (ll ++ lr) -> i < s ->
-  low <= size ll < high -> low <= size lr < high -> low <= size r < high ->
-  wf_dtree_l (balanceL' Black (delete_leaves Red ll lr i) (Bleaf _ r)).
-Proof.
-  move=> ic ? wfll wflr wfr.
-  by rewrite balanceL'_wf // delete_leaves_wf //= -!size_cat -(eqP ic).
-Qed.
-
-Lemma stay_wfR l rl rr i ls:
-  ls == size l -> i < size l + size rl + size rr ->
-  low <= size l < high -> low <= size rl < high -> low <= size rr < high ->
-  wf_dtree_l (balanceR' Black (Bleaf _ l) (delete_leaves Red rl rr (i - ls))).
-Proof.
-  move=> ic ? wfl wfrl wfrr.
-  rewrite balanceR'_wf // delete_leaves_wf //= ltn_subLR ?addnA ?(eqP ic) //.
-  apply /(leq_trans (leq_trans Hlow1 _) (leq_addr _ _)); by decomp wfrl.
 Qed.
 
 Lemma ddel_wf (B : dtree) n i :
-  n > 0 ->
-  is_redblack B Black n ->
+  0 < n ->
   i < dsize B ->
+  is_redblack B Black n ->
   wf_dtree_l B ->
-  wf_dtree_l (ddel B i).
+  wf_dtree_l (ddel B i : deleted_dtree).
 Proof.
-  move: n; functional induction (ddel B i) => n n_gt0 rbB Hi wf.
-  - by rewrite delete_leaves_wf //; decomp wf.
-  - by rewrite delete_leaves_wf //; decomp wf.
-  - apply /stay_wfL; move: e0; by decomp wf.
-  - apply /stay_wfR; by decomp wf.
-  - apply /stay_wfL; move: e0; decomp wf; by rewrite ?size_cat.
-  - apply /stay_wfR; decomp wf; by rewrite -?addnA.
-  - rewrite balanceL'_wf // ?(IHd n.-1) //; decomp rbB => //=.
-        rewrite (leq_trans e0) //; decomp wf => //=.
-        by rewrite size_cat -!dsizeE' // leq_addr.
-      decomp wf; by rewrite !(dsizeE',donesE',size_cat,count_cat,eqxx).
-    by decomp wf.
-  - rewrite balanceR'_wf // ?(IHd n.-1) //; decomp rbB => //=; decomp wf => //.
-    rewrite ltn_subLR ?size_cat -?dsizeE' //.
-    by rewrite (leq_trans (dsize_gt0 H13)) // leq_addr.
-  - rewrite balanceL'_wf // ?(IHd n.-1) //; decomp rbB => //=; decomp wf => //.
-    by rewrite !dsizeE' // -size_cat -(eqP H5).
-  - rewrite balanceR'_wf // ?(IHd n.-1) //; decomp rbB => //=; decomp wf => //.
-      rewrite ltn_subLR ?size_cat -?dsizeE' //; first by rewrite addnA.
-      by rewrite (leq_trans (dsize_gt0 H10)) // leq_addr.
-    by rewrite !(dsizeE',donesE',eqxx).
-  - case: c y rbB Hi wf => //= y; move/andP => [] rbl rbr sc.
-      move/andP => [/eqP H] /andP [?] /andP [wfl wfr].
-      rewrite balanceL'_wf // (IHd n) // ?is_redblack_Red_Black //.
-      by rewrite dsizeE' // -H.
-    move/andP: rbl => [] _ rbl /andP[/eqP H] /andP[los] /andP[wfl wfr].
-    case: n n_gt0 rbl rbr => // n; case neq: n => /= n_gt0.
-      move: l y sc wfl IHd H los => [[]//ll[]?? lr|?] //;
-      move: r wfr => [[]//rl[]?? rr|?] //;
-      try move:ll lr =>[[]//|?] [[]//|?] //=;
-      try move:rl rr =>[[]//|?] [[]//|?] //=.
-      rewrite !size_cat // => wfr _ ? wfl ? H ? _ _.
-      rewrite balanceL'_wf // ddel0E delete_leaves_wf //; first (by rewrite -H);
-        by decomp wfl.
-    move=>rbl rbr; by rewrite balanceL'_wf // (IHd n) // ?neq // dsizeE' // -H.
-  - case: c y rbB Hi wf => //= y; move/andP => [] rbl rbr sc;
-      move/andP => [/eqP H] /andP [los] /andP [wfl wfr].
-      rewrite balanceR'_wf // (IHd n) // ?is_redblack_Red_Black //.
-      by rewrite ltn_subLR // ?H -?dsizeE' // dsize_gt0.
-    move/andP: rbl => [] _ rbl.
-    case: n n_gt0 rbl rbr => // n; case neq: n => /= n_gt0.
-      move: l y sc wfl IHd H los => /= [[]//ll[]?? lr|?] //;
-      move: r wfr => [[]//rl[]?? rr|?] //;
-      try move:ll lr =>[[]//|?] [[]//|?] //=;
-      try move:rl rr =>[[]//|?] [[]//|?] //=.
-      rewrite !size_cat // => wfr _ ? wfl ? H ? _ _.
-      rewrite balanceR'_wf //= ddel0E delete_leaves_wf //; decomp wfr => //.
-      by rewrite H ltn_subLR // (leq_trans Hlow1) // (leq_trans H2) // leq_addr.
-    move=>rbl rbr; rewrite balanceR'_wf // (IHd n) // ?neq // dsizeE' //.
-    by rewrite H ltn_subLR // -!dsizeE' // dsize_gt0.
-  - by case: n n_gt0 rbB.
+  move => Hn Hi rbB wfB; rewrite dsizeE' // in Hi; move: Hn Hi rbB wfB.
+  rewrite /= /lt_index /right_index /=.
+  elim: B n i => [[] l IHl [??] r IHr|?] n i Hn Hi rbB wfB /=;
+    last by move/eqP: rbB Hn => /= ->.
+  + case: ifP => Hc;
+    case: l r Hi rbB IHl IHr wfB =>
+        [[]?[??]?|?] [[]?[??]?|?]// Hi rbB IHl IHr wfB;
+    rewrite ?(balanceL'_wf, balanceR'_wf,
+              IHl n, IHr n, delete_from_leaves_wf, ltn_subLR) //;
+    move: rbB wfB Hi Hc;
+    do! (decompose_rewrite; rewrite /= ?size_cat) => //;
+    rewrite ?(ltn_addr, dsize_gt0, leq_trans Hlow1) //=.
+  + case: n Hn rbB => [//|[|n]] Hn rbB.
+  * case: l r Hi rbB IHl IHr wfB =>
+        [[] [[]//|?] [??] [[]//|?]|?] [[] [[]//|?] [??] [[]|?]|?] //=
+        Hi rbB IHl IHr wfB;
+      try case: ifP => Hc;
+      rewrite ?(balanceL'_wf, balanceR'_wf, delete_from_leaves_wf) //;
+      try move: Hc; move: wfB rbB Hi;
+      do! (decompose_rewrite; rewrite /= ?size_cat //).
+    - by rewrite ltn_subLR // ltn_addr // (leq_trans Hlow1).
+    - by rewrite ltn_subLR ?addnA // ltn_addr // (leq_trans Hlow1).
+    - by rewrite -ltn_subLR // (leq_trans Hlow1).
+    - by rewrite ltn_subLR // ltn_addr // (leq_trans Hlow1).
+  * time (case:l r Hi rbB IHl IHr wfB =>
+        [[] ll [??] lr|?] [[]?[??]?|?] Hi rbB IHl IHr wfB;
+      last rewrite delete_from_leaves_wf //;
+      case: ifP => Hc //;
+      try case: ll lr IHl rbB wfB Hi => [[]???|?] [[]???|?] // IHl rbB wfB Hi;
+      rewrite ?(balanceL'_wf, balanceR'_wf,
+                IHl n.+1, IHr n.+1, delete_from_leaves_wf, ltn_subLR) //;
+      move: rbB wfB Hi Hc;
+      do! (decompose_rewrite; rewrite /= ?size_cat) => //;
+      by rewrite ?(ltn_addr, dsize_gt0, leq_trans Hlow1)).
 Qed.
 
 Lemma ddel_wf' (B : dtree) n i :
   is_redblack B Black n ->
   i < dsize B ->
   wf_dtree' B ->
-  wf_dtree' (ddel B i : dtree).
+  wf_dtree' ((ddel B i : deleted_dtree) : dtree).
 Proof.
 case: n => [|n].
   case: B => [[]// [[]//???|s1] [n1 o1] [[]//???|s2]|s] //=.
-    rewrite ddel0E => _ Hi wf.
-    apply /wf_dtree_dtree' /delete_leaves_wf => //; by decomp wf.
+    move => _ Hi wf.
+    apply /wf_dtree_dtree' /delete_from_leaves_wf => //; by decomp wf.
   move=> _ Hi Hs; rewrite size_delete //.
   by rewrite (ltn_predK Hi) ltnW.
 case: B => // c l d r rb Hi wf.
 by apply /wf_dtree_dtree' /(@ddel_wf _ n.+1).
 Qed.
 
-End delete.
+End ddelete.
